Examples/Code_haskell.thy
@@ -95,6 +95,6 @@ export_code Rule
   to_simple_firewall_without_interfaces
   sanity_wf_ruleset
   (*spoofing:*) example_TUM_i8_spoofing_ipassmt no_spoofing_iface ipassmt_sanity_defined map_of_ipassmt
-  in Haskell module_name "Network.IPTables.Generated" file "tmp/"
+  in Haskell module_name "Network.IPTables.Generated" file "generated_code/"
 
 end
